chore: add basic pointer chasing example, next build BDDs on top of it
Also add hash-consing support, to enable auto-hash-consing as a policy.

PointerChase/Basic.lean
@@ -4,11 +4,33 @@
 import Std
 open Std
 
-namespace Bdd
+namespace PointerChase
 
+/-- The (polynomial) functor of the data we want to store, parametrized by the pointer locations -/
 inductive NodeF (α : Type) (f : Type) where
 | value (value : Bool)
 | var (a : α) (low high : f)
+
+instance : Functor (NodeF α) where
+  map f
+  | .value v => .value v
+  | .var a low high => .var a (f low) (f high)
+
+
+def ValueNode α := NodeF α Unit
+
+/-- The value of the node, without any of the pointer information we attach to it. -/
+def NodeF.toValueNode : NodeF α f → ValueNode α := Functor.map (fun _ => ())
+
+@[simp]
+theorem NodeF.toValueNode_value {α f : Type} (v : Bool) : (@NodeF.value α f v).toValueNode = NodeF.value v := rfl
+
+@[simp]
+theorem NodeF.toValueNode_var {α f : Type} {a} {low high} : (@NodeF.var α f a low high).toValueNode = NodeF.var a () () := rfl
+
+/-- Coerce any node to a value node, that forgets the pointer data. -/
+instance : CoeOut (NodeF α f) (ValueNode α) where
+  coe := NodeF.toValueNode
 
 /-- A Node has fields as natural numbers. -/
 abbrev PreNode α := NodeF α Nat
@@ -257,7 +279,7 @@ def Nodes.Inode.toPreNode {α : Type} {nodes : Nodes α} (n : nodes.Inode) : Pre
   | .var a low high => NodeF.var a low.ix high.ix
 
 @[simp]
-theorem Nodes.Inode.toPreNode_inbounds {α : Type} {nodes : Nodes α} (n : nodes.Inode) :
+theorem Nodes.Inode_inboundes {α : Type} {nodes : Nodes α} (n : nodes.Inode) :
   n.toPreNode.LessThan nodes.heap.size := by
   cases n
   case value v =>
@@ -301,122 +323,32 @@ def Nodes.insert (nodes : Nodes α) (n : nodes.Inode) : Nodes.insert.Result α :
     simp
   ⟨nodes', ptr⟩
 
+/-- Grabbing the values gives us equal results -/
 @[simp]
 theorem Nodes.val_ptr_insert_eq
   (nodes : Nodes α) (n : nodes.Inode) :
-  (nodes.insert n).ptr.val.toPreNode = n.toPreNode := by
+  (nodes.insert n).ptr.val.toValueNode = n.toValueNode := by
   simp [Nodes.insert, Nodes.Ptr.val, Nodes.lastPtr]
   split
   case h_1 v heq =>
     simp [Array.size_push] at heq
-    sorry
+    cases n
+    case value v =>
+      simp [Inode.toPreNode] at heq
+      subst v
+      simp [NodeF.toValueNode]
+      rfl
+    case var v lo hi =>
+      simp [Inode.toPreNode] at heq
   case h_2 v heq =>
     simp [Array.size_push] at heq
-    sorry
+    cases n
+    case value v =>
+      simp [Inode.toPreNode] at heq
+    case var v lo hi =>
+      simp [Inode.toPreNode] at heq
+      obtain ⟨s1, _, _⟩ := heq
+      subst s1 
+      simp
 
-
-
-/-- A BDD, represented as a tree -/
-inductive Tree
-| value (value : Bool)
-| var (low high : Tree)
-deriving DecidableEq, Hashable, Inhabited
-
-def Tree.mkFalse : Tree := Tree.value false
-
-namespace Node
-
-
-/--
-A node is irredundant if either it's not a variable node,
-or if it is a variable node, then the low and high nodes are different.
--/
-def NoSameChildren (n : Node α) : Prop :=
-  ∀ {a low high}, n = .var a low high → low ≠ high
-
-end Node
-
-def Ordered (nodes : Array (Node α)) : Prop :=
-  ∀ {i a low high} (hi : i < nodes.size),
-     nodes[i] = .var a low high → (low < i) ∧ (high < i)
-
-@[simp]
-def Ordered_empty : Ordered (#[] : Array (Node α)) := by
-  intros i _a low high hi _hnode
-  cases hi
-
-def Cache (α : Type) [DecidableEq α] [Hashable α] : Type :=
-  HashMap (Node α) Nat
-
-def Cache.empty {α : Type} [DecidableEq α] [Hashable α] : Cache α := HashMap.empty
-
-inductive Cache.WF (α : Type) [DecidableEq α] [Hashable α] :
-    (cache : Cache α) → (nodes : Array (Node α)) → Prop where
-/-- The empty cache is always well formed -/
-| empty : Cache.WF α (Cache.empty) nodes
-
-structure RODD (α : Type) [DecidableEq α] [Hashable α] where
-  nodes : Array (Node α)
-  cache : Cache α
-
-/-- A handle to a canonicalized node in the RODD hash map. -/
-partial def RODD.canonNode [DecidableEq α] [Hashable α]
-  (n : Node α) (rodd : RODD α) : Node α := Id.run do
-  match n with
-  | .value v =>
-    /- TODO: prove that this can't happen -/
-    -- We can show that we will never use the default value.
-    let .some ix := rodd.cache.get? n | return n
-    rodd.nodes.getD ix n
-  | .var a low high =>
-     let low := RODD.canonNode <| rodd.nodes[low]!
-     let high := RODD.canonNode <| rodd.nodes[high]!
-
-
-
-
-def RODD.empty {α : Type} [DecidableEq α] [Hashable α] : RODD α := {
-  nodes := #[],
-  cache := HashMap.empty,
-  }
-
-namespace RODD
-
-variable {α : Type} [DecidableEq α] [Hashable α] {m : Type → Type} [Monad m]
-def postorderAt (nodes : Array (Node α)) (ordered : Ordered nodes) (fvar : σ → Bool → m σ) (fnode : (init : σ) → (a : α) →  (lo : σ) → (hi : σ) → m σ)
-    (init : σ) (ix : Nat) (hix : ix < nodes.size) : m σ := do
-  match hnode : nodes[ix] with
-  | .value v => fvar init v
-  | .var a lo hi =>
-    have := ordered hix hnode
-    let loVal ← postorderAt nodes ordered fvar fnode init lo (by omega)
-    let hiVal ← postorderAt nodes ordered fvar fnode init hi (by omega)
-    fnode init a loVal hiVal
-
-/-- Postorder traversal of BDD -/
-def postorder (d : RODD α) (init : σ)
-    (fvar : σ → Bool → m σ) (fnode : (init : σ) → (a : α) → (lo : σ) → (hi : σ) → m σ)  : m σ := do
-  if h : d.nodes.size = 0
-  then return init
-  else postorderAt d.nodes d.ordered fvar fnode init (d.nodes.size-1) (by omega)
-
-/-- Convert the subDAG into a tree. -/
-def treeAt {ix: Nat} (nodes : Array (Node α)) (ordered : Ordered nodes) (hix : ix < nodes.size): Tree :=
-  Id.run <| postorderAt nodes ordered
-    (fvar := fun _ v => return Tree.value v)
-    (fnode := fun _  _ lo hi => return Tree.var lo hi)
-    Tree.mkFalse ix hix
-
-/- An empty RODD. -/
-def RODD.empty {α : Type} [DecidableEq α] [Hashable α] : RODD α := {
-  nodes := #[],
-  cache := HashMap.empty,
-  ordered := by simp,
-}
-
-
-namespace Node
-end Node
-
-
-end Bdd
+end PointerChase
