Examples.lean
@@ -1,0 +1,5 @@
+import PointerChase.Basic
+import Examples.BDD
+
+def main : IO Unit :=
+  IO.println s!"Hello"
