Examples/BDD.lean
@@ -1,0 +1,108 @@
+import PointerChase.Basic
+-- Little engines of proof, lecture 4
+
+-- https://www.csl.sri.com/people/shankar/LEP/LEP5.pdf
+
+/-
+/-- A BDD, represented as a tree -/
+inductive Tree
+| value (value : Bool)
+| var (low high : Tree)
+deriving DecidableEq, Hashable, Inhabited
+
+def Tree.mkFalse : Tree := Tree.value false
+
+namespace Node
+
+
+/--
+A node is irredundant if either it's not a variable node,
+or if it is a variable node, then the low and high nodes are different.
+-/
+def NoSameChildren (n : Node α) : Prop :=
+  ∀ {a low high}, n = .var a low high → low ≠ high
+
+end Node
+
+def Ordered (nodes : Array (Node α)) : Prop :=
+  ∀ {i a low high} (hi : i < nodes.size),
+     nodes[i] = .var a low high → (low < i) ∧ (high < i)
+
+@[simp]
+def Ordered_empty : Ordered (#[] : Array (Node α)) := by
+  intros i _a low high hi _hnode
+  cases hi
+
+def Cache (α : Type) [DecidableEq α] [Hashable α] : Type :=
+  HashMap (Node α) Nat
+
+def Cache.empty {α : Type} [DecidableEq α] [Hashable α] : Cache α := HashMap.empty
+
+inductive Cache.WF (α : Type) [DecidableEq α] [Hashable α] :
+    (cache : Cache α) → (nodes : Array (Node α)) → Prop where
+/-- The empty cache is always well formed -/
+| empty : Cache.WF α (Cache.empty) nodes
+
+structure RODD (α : Type) [DecidableEq α] [Hashable α] where
+  nodes : Array (Node α)
+  cache : Cache α
+
+/-- A handle to a canonicalized node in the RODD hash map. -/
+partial def RODD.canonNode [DecidableEq α] [Hashable α]
+  (n : Node α) (rodd : RODD α) : Node α := Id.run do
+  match n with
+  | .value v =>
+    /- TODO: prove that this can't happen -/
+    -- We can show that we will never use the default value.
+    let .some ix := rodd.cache.get? n | return n
+    rodd.nodes.getD ix n
+  | .var a low high =>
+     let low := RODD.canonNode <| rodd.nodes[low]!
+     let high := RODD.canonNode <| rodd.nodes[high]!
+
+
+
+
+def RODD.empty {α : Type} [DecidableEq α] [Hashable α] : RODD α := {
+  nodes := #[],
+  cache := HashMap.empty,
+  }
+
+namespace RODD
+
+variable {α : Type} [DecidableEq α] [Hashable α] {m : Type → Type} [Monad m]
+def postorderAt (nodes : Array (Node α)) (ordered : Ordered nodes) (fvar : σ → Bool → m σ) (fnode : (init : σ) → (a : α) →  (lo : σ) → (hi : σ) → m σ)
+    (init : σ) (ix : Nat) (hix : ix < nodes.size) : m σ := do
+  match hnode : nodes[ix] with
+  | .value v => fvar init v
+  | .var a lo hi =>
+    have := ordered hix hnode
+    let loVal ← postorderAt nodes ordered fvar fnode init lo (by omega)
+    let hiVal ← postorderAt nodes ordered fvar fnode init hi (by omega)
+    fnode init a loVal hiVal
+
+/-- Postorder traversal of BDD -/
+def postorder (d : RODD α) (init : σ)
+    (fvar : σ → Bool → m σ) (fnode : (init : σ) → (a : α) → (lo : σ) → (hi : σ) → m σ)  : m σ := do
+  if h : d.nodes.size = 0
+  then return init
+  else postorderAt d.nodes d.ordered fvar fnode init (d.nodes.size-1) (by omega)
+
+/-- Convert the subDAG into a tree. -/
+def treeAt {ix: Nat} (nodes : Array (Node α)) (ordered : Ordered nodes) (hix : ix < nodes.size): Tree :=
+  Id.run <| postorderAt nodes ordered
+    (fvar := fun _ v => return Tree.value v)
+    (fnode := fun _  _ lo hi => return Tree.var lo hi)
+    Tree.mkFalse ix hix
+
+/- An empty RODD. -/
+def RODD.empty {α : Type} [DecidableEq α] [Hashable α] : RODD α := {
+  nodes := #[],
+  cache := HashMap.empty,
+  ordered := by simp,
+}
+
+
+namespace Node
+end Node
+-/
