Main.lean
@@ -1,4 +1,0 @@
-import Bdd.Basic
-
-def main : IO Unit :=
-  IO.println s!"Hello, {hello}!"
